abstract exp

proof/examples/zk/multlimb/W64_exp_proof_4.ec
@@ -4,8 +4,7 @@ require import JModel.
 require import BitEncoding.
 import BS2Int.
 
-require import Fp_small.
-require import Fp_small_proof.
+require import Zp_big.
 require import W64_exp_proof_1.
 require import W64_exp_proof_2.
 require import W64_exp_proof_3.
@@ -15,18 +14,19 @@ import IterOp.
 
 
 
-
+print W64x4.
 module M4 = {
 
-    proc expm (x:W64.t, n:W64.t) : W64.t = {
+    proc expm (x:R, n:R) : R = {
     
-    var x1, x2, x3, x4, bit, d, p, par : W64.t;
+    var x1, x2, x3, x4, bit : R;
+    var par, p, d : W64.t;
     var ctr:int;
 
-    d <- ith_bitword64 n (W64.size - 1);
-    (x1,x2,x3, x4) <- (W64.one,W64.one,x,x *** x);
+    d <- ith_bitR n (256 - 1);
+    (x1,x2,x3, x4) <- (oneR,oneR,x,x *** x);
 
-    ctr <- W64.size - 1;
+    ctr <- 256 - 1;
     p <- d;
     (x1,x3) <- as_bool d ? (x3,x1) : (x1,x3);
     (x2,x4) <- as_bool d ? (x4,x2) : (x2,x4);
@@ -34,36 +34,38 @@ module M4 = {
     while (0 < ctr) {
       ctr <- (ctr - 1);
       p <- d;
-      d <-  d `|` ith_bitword64 n ctr;
-      par <- ith_bitword64 n (ctr + 1) `^` ith_bitword64 n ctr;
+      d <-  d `|` ith_bitR n ctr;
+      par <- ith_bitR n (ctr + 1) `^` ith_bitR n ctr;
       (x1,x2) <- if as_bool par then (x2,x1) else (x1, x2);
       x1 <- x1 *** x2;
       x2 <- x2 *** x2;
       (x1,x3) <- as_bool (d `^` p) ? (x3,x1) : (x1,x3);
       (x2,x4) <- as_bool (d `^` p)  ? (x4,x2) : (x2,x4);
     }
-    (x1,x2) <- if ! as_bool (ith_bitword64 n 0)  then (x2,x1) else (x1, x2);    
+    (x1,x2) <- if ! as_bool (ith_bitR n 0)  then (x2,x1) else (x1, x2);    
     return x1;
   }  
 
 
 }.
 
+
 axiom qqq n x :
-  ith_bitlist (W64.w2bits n) x = ith_bitword64 n x.
+  ith_bitlist (Rbits n) x = ith_bitR n x.
 
 
-axiom www n x : size n = 64 =>
-  ith_bitlist n x = ith_bitword64 (W64.bits2w n) x.
+axiom www n x : size n = 256 =>
+  ith_bitlist n x = ith_bitR (bitsR n) x.
 
+axiom iii n : size (Rbits n) = 256.
 
 lemma exp_3_4_1 :
- equiv[ M3.expm ~ M4.expm : arg{1}.`1 = arg{2}.`1 /\ (W64.bits2w arg.`2{1}) = (arg.`2{2})  /\ size n{1} = 64 /\  0 < size n{1} ==> ={res}].
+ equiv[ M3.expm ~ M4.expm : arg{1}.`1 = arg{2}.`1 /\ (bitsR arg.`2{1}) = (arg.`2{2})  /\ size n{1} = 256 /\  0 < size n{1} ==> ={res}].
 proc.
 wp.
 while (={ctr,  x1,x2,  x3, x4, d, p}  
-   /\ W64.bits2w n{1} = n{2}
-   /\ size n{1} = 64).
+   /\ bitsR n{1} = n{2}
+   /\ size n{1} = 256).
 wp. skip. progress. 
 smt (qqq www).
 smt (qqq www).
@@ -87,12 +89,12 @@ qed.
 
 
 lemma exp_3_4_2 :
- equiv[ M3.expm ~ M4.expm : arg{1}.`1 = arg{2}.`1 /\ (arg.`2{1}) = (W64.w2bits arg.`2{2})    /\  0 < size n{1} ==> ={res}].
+ equiv[ M3.expm ~ M4.expm : arg{1}.`1 = arg{2}.`1 /\ (arg.`2{1}) = (Rbits arg.`2{2})    /\  0 < size n{1} ==> ={res}].
 proc.
 wp.
 while (={ctr,  x1,x2,  x3, x4, d, p}  
-   /\ n{1} = W64.w2bits n{2}
-   /\ size n{1} = 64).
+   /\ n{1} = Rbits n{2}
+   /\ size n{1} = 256).
 wp. skip. progress. 
 smt (qqq www).
 smt (qqq www).
@@ -101,14 +103,16 @@ smt (qqq www).
 smt (qqq www).
 wp. 
 skip. 
-progress.
-smt (qqq www).
-smt (qqq www).
-smt (qqq www).
-smt (qqq www).
-smt (qqq www).
-smt (qqq www).
-
+progress.  rewrite iii. auto.
+smt (qqq www iii).
+smt (qqq www iii).
+smt (qqq www iii).
+smt (qqq www iii).
+smt (qqq www iii).
+smt (qqq www iii).
+smt (qqq www iii).
+smt (qqq www iii).
+smt (qqq www iii).
 qed.
 
 
