proof/examples/zk/abstract/Abstract_exp_proof_1.ec
@@ -1,0 +1,286 @@
+require import AllCore IntDiv CoreMap List.
+
+require import JModel.
+require import BitEncoding.
+import BS2Int.
+
+type R.
+
+
+module type BasicOps = {
+  proc ith_bit (r : R, p : W64.t) : W64.t
+  proc mulm (p : R, a : R, b : R) : R
+  proc swapr (a : R, b : R, c : W64.t) : R * R
+}.
+
+type bits = bool list.
+
+
+op tonat : bits -> int = bs2int.
+op ith_bit (n : bits) (x : int) : bool = nth witness n x.
+op has_true (bs : bits) : bool = has (fun x => x = true) bs.
+
+op P : int.
+op ( *** ) (a b : R) : R.
+op (^) (x : R) (n : int) : R.
+op oneR : R.
+op Rsize : int.
+op Rbits (r : R) : bits.
+op bitsR (r : bits) : R.
+op as_w64 (x : bool) : W64.t  = x ? W64.one : W64.zero.
+op ith_bitR (r : R) (x : int) : W64.t = as_w64 (ith_bit (Rbits r) x).
+op as_bool (x : W64.t) : bool  = (x = W64.one).
+op ith_bitlist (n : bits) (x : int)  : W64.t = as_w64 (ith_bit n x).
+op valR (x : R) : int = tonat (Rbits x).
+op ImplR (p : R) (P : int) = (valR p = P).
+
+
+axiom P_prime: prime P.
+axiom qqq n x : ith_bitlist (Rbits n) x = ith_bitR n x.
+axiom www n x : size n = Rsize => ith_bitlist n x = ith_bitR (bitsR n) x.
+axiom iii n : size (Rbits n) = Rsize.
+axiom Rsize_max : Rsize < W64.max_uint.
+axiom Rsize_pos : 0 < Rsize.
+axiom prop1   : tonat[true] = 1.
+axiom prop2   : tonat[false] = 0.
+axiom prop3 s : tonat (true :: s) = 2 * (tonat s) + 1.
+axiom prop4 s : tonat (false :: s) = 2 * (tonat s).
+axiom prop5 s : 0 <= tonat s.
+axiom exp_prop1 x : x ^ 0 = oneR.
+axiom exp_prop2 x : x ^ 1 = x.
+axiom exp_prop3 (x : R) (a b : int) :  x ^ (a + b) = x ^ a *** x ^ b.
+axiom exp_prop4 (x : R) (a b : int) :  x ^ (a * b) = (x ^ a) ^ b.
+axiom exp_prop5 (x : R) :  x *** oneR = x.
+axiom exp_prop6 (a b c : R) :  (a *** b) *** c = a *** (b *** c).
+axiom exp_prop7 (a b : R) :  (a *** b) = b *** a.
+axiom to_uintP: forall (x y : R), valR (x *** y) = valR x * valR y %% P.
+axiom rsize_prop (r : R) : size (Rbits r) = Rsize.
+axiom bitsR_prop a b : tonat a = valR b => size a = Rsize => bitsR a = b.
+axiom valR_one : valR oneR = 1.
+
+
+
+(* Embedding into ring theory *)
+require ZModP.
+clone import ZModP.ZModField as Zp with
+        op p <= P
+        rename "zmod" as "zp"
+        proof prime_p by exact P_prime.
+
+op (^^) (x : zp)(n : int) : zp = inzp (asint x ^ n).
+
+abbrev ImplFp x y = valR x = asint y.
+
+module Spec = {
+  proc ith_bit(r : R, ctr : int) = { 
+    return (ith_bitR r ctr);
+  }
+  proc mul(a : R, b : R) = { 
+    return (a *** b);
+  }
+
+  proc swapr(a : R, b : R, c : bool) = { 
+    return c ? (b,a) : (a, b);
+  }
+
+ proc mulm(a b: zp): zp = {
+    var r;
+    r <- a * b;
+    return r;
+ }
+
+ proc expm(a : zp,  b: int): zp = {
+    var r;
+    r <- a ^^ b;
+    return r;
+ }
+
+}.
+
+lemma hast3 xs :  0 < size xs => drop (size xs - 1) xs = [ith_bit xs (size xs - 1) ].
+progress. rewrite (drop_nth witness). progress. smt(). smt().
+simplify. smt(@List).
+qed.
+    
+lemma hast2 xs :  0 < size xs => ith_bit xs (size xs - 1) = has_true (drop (size xs - 1) xs).
+progress. rewrite hast3;auto. smt().
+qed.
+
+lemma hast1 : forall xs ctr, 0 <= ctr -1 < size xs
+  => (has_true (drop ctr xs) || ith_bit xs (ctr - 1)) = has_true (drop (ctr - 1) xs).
+progress. 
+rewrite ( drop_nth witness (ctr - 1) ). progress. smt(). 
+qed.
+
+
+lemma hast5  : forall xs, ! (has_true xs) => (bs2int xs) = 0.
+elim. smt. smt. qed.
+
+
+lemma hast4  : forall xs (x : R), ! (has_true xs) => x ^ (tonat xs) = oneR.
+progress. rewrite /tonat. rewrite hast5. auto.
+rewrite /(^). simplify. smt.
+qed.
+
+lemma hast6  : forall xs (x : int), ! (has_true xs) => x ^ (tonat xs) = 1.
+progress. rewrite /tonat. rewrite hast5. auto.
+smt.
+qed.
+
+
+
+module M1 = {
+
+  proc expm_spec (x:R, n:bits) : R = {
+    return x ^ (tonat n); 
+  }  
+
+  proc expm_naive (x:R, n:bits) : R = {
+    
+    var x1, x2, x3, x4 : R;
+    var ctr:int;
+    var bit, d, p :bool;    
+    d <- ith_bit n (size n - 1);
+    (x1,x2,x3, x4) <- (oneR,oneR,x,x *** x);
+
+    ctr <- size n - 1;
+    p <- d;
+    (x1,x3) <- d ? (x3,x1) : (x1,x3);
+    (x2,x4) <- d ? (x4,x2) : (x2,x4);
+
+    while (0 < ctr) {
+      ctr <- (ctr - 1);
+      p <- d;
+      d <- d || ith_bit n ctr;
+      (x1,x2) <- (ith_bit n ctr) ? ((x1***x2), (x2***x2)) : ((x1***x1), (x1***x2));
+      (x1,x3) <- d ^ p ? (x3,x1) : (x1,x3);
+      (x2,x4) <- d ^ p ? (x4,x2) : (x2,x4);
+    }
+    return x1;
+  }  
+}.
+
+
+
+lemma exp_naive_correct xx nn : 
+  equiv[ M1.expm_naive ~ M1.expm_spec : ={arg} /\ arg{1} = (xx, nn){1} /\  0 < size nn ==> ={res}].
+proof. proc. 
+while {1} (d{1} = has_true (drop ctr n) /\ ctr < size n /\ (has_true (drop ctr n) =>
+  (x1 = x ^ tonat (drop ctr n) 
+    /\ x2 = x1 *** x  /\ (x3,x4){1} = (oneR, oneR)) ) /\ (!has_true (drop ctr n) => x1 = oneR /\ x2 = oneR /\ x3 = x /\ x4 = x *** x) ){1} (ctr{1}). 
+progress.
+wp. skip.  progress. 
+rewrite (drop_nth witness (ctr{hr} - 1)). smt(). simplify. rewrite /ith_bit. smt().
+smt(). 
+case (ith_bit n{hr} (ctr{hr} - 1 )). progress.
+  case (!has_true (drop ctr{hr} n{hr})). move => casef.  
+   rewrite casef.
+  have -> : true ^ false  = true. smt(@Bool). simplify.
+  have -> : x3{hr} = x{hr}. smt(). 
+  have -> : (drop (ctr{hr} - 1) n{hr}) = true :: (drop (ctr{hr} ) n{hr}).  
+  rewrite (drop_nth witness (ctr{hr} - 1)).  smt(). smt().
+   rewrite /tonat. 
+rewrite  bs2int_cons.
+rewrite /b2i. simplify.
+have -> : x{hr} ^ (1 + 2 * bs2int (drop ctr{hr} n{hr}))
+  = x{hr} *** x{hr} ^ (2 * bs2int (drop ctr{hr} n{hr})).
+rewrite exp_prop3. rewrite exp_prop2. auto.
+have ->: x{hr} ^ (2 * bs2int (drop ctr{hr} n{hr}))
+ = x{hr} ^ (bs2int (drop ctr{hr} n{hr})) *** x{hr} ^ (bs2int (drop ctr{hr} n{hr})).
+smt.
+have -> : bs2int (drop ctr{hr} n{hr})  = 0.
+rewrite  hast5. auto. auto. rewrite exp_prop1. rewrite exp_prop5. rewrite exp_prop5. auto.
+simplify.
+move => casef. rewrite casef. 
+  have -> : true ^ true  = false. smt(@Bool). simplify.
+  have -> : (drop (ctr{hr} - 1) n{hr}) = true :: (drop (ctr{hr} ) n{hr}).  
+  rewrite (drop_nth witness (ctr{hr} - 1)). 
+progress. smt().
+smt(). 
+simplify.
+rewrite /ith_bit in H4. rewrite H4. auto.
+rewrite prop3. 
+have -> : x1{hr} *** x2{hr} = x{hr} ^ tonat (drop ctr{hr} n{hr}) *** x{hr} ^ tonat (drop ctr{hr} n{hr}) *** x{hr}.
+rewrite H0. auto.
+rewrite H0. auto. 
+rewrite H0. auto.  
+pose n := tonat (drop ctr{hr} n{hr}).
+smt (exp_prop6).
+pose n := tonat (drop ctr{hr} n{hr}).
+rewrite exp_prop3. rewrite exp_prop2. smt.
+progress.
+have z: has_true (drop ctr{hr} n{hr}) = true. 
+have x : drop (ctr{hr} - 1) n{hr} = ith_bit n{hr} (ctr{hr} - 1) :: drop ctr{hr} n{hr}.
+rewrite (drop_nth witness (ctr{hr} - 1)).  smt(). rewrite H4.
+simplify. rewrite - H4. rewrite /ith_bit. auto.
+smt.
+rewrite z.
+have -> : true ^ true  = false. smt(@Bool). simplify.
+have -> : x1{hr} *** x1{hr} = x{hr} ^ tonat (drop ctr{hr} n{hr}) *** x{hr} ^ tonat (drop ctr{hr} n{hr}).
+smt. 
+rewrite (drop_nth witness (ctr{hr} - 1)).  smt(). smt.
+have -> : (has_true (drop ctr{hr} n{hr}) || ith_bit n{hr} (ctr{hr} - 1)) = true.
+rewrite (hast1 n{hr} ctr{hr} _). progress. smt().
+smt(). rewrite H3. auto.
+case (has_true (drop ctr{hr} n{hr})). progress. 
+have -> : true ^ true = false. smt().
+simplify. 
+case ( ith_bit n{hr} (ctr{hr} - 1)).
+progress. rewrite H0. auto.
+rewrite H0. auto. rewrite H0. auto.
+smt(exp_prop1 exp_prop2 exp_prop3 exp_prop4 exp_prop5 exp_prop6).
+smt(exp_prop1 exp_prop2 exp_prop3 exp_prop4 exp_prop5 exp_prop6).
+progress.
+smt(exp_prop1 exp_prop2 exp_prop3 exp_prop4 exp_prop5 exp_prop6).
+rewrite hast1. smt(). rewrite H3.
+case (has_true (drop ctr{hr} n{hr})).
+progress.
+smt(exp_prop1 exp_prop2 exp_prop3 exp_prop4 exp_prop5 exp_prop6).
+smt(exp_prop1 exp_prop2 exp_prop3 exp_prop4 exp_prop5 exp_prop6).
+
+rewrite hast1. smt(). rewrite H3.
+case (has_true (drop ctr{hr} n{hr})).
+progress.
+smt(exp_prop1 exp_prop2 exp_prop3 exp_prop4 exp_prop5 exp_prop6).
+smt(exp_prop1 exp_prop2 exp_prop3 exp_prop4 exp_prop5 exp_prop6).
+
+rewrite hast1. smt(). rewrite H3.
+case (has_true (drop ctr{hr} n{hr})).
+progress.
+smt(exp_prop1 exp_prop2 exp_prop3 exp_prop4 exp_prop5 exp_prop6).
+smt(exp_prop1 exp_prop2 exp_prop3 exp_prop4 exp_prop5 exp_prop6).
+rewrite hast1. smt(). rewrite H3.
+case (has_true (drop ctr{hr} n{hr})).
+progress.
+smt(exp_prop1 exp_prop2 exp_prop3 exp_prop4 exp_prop5 exp_prop6).
+smt(exp_prop1 exp_prop2 exp_prop3 exp_prop4 exp_prop5 exp_prop6).
+rewrite hast1. smt(). rewrite H3.
+smt.
+rewrite hast1. smt(). rewrite H3.
+smt.
+smt().
+wp.  skip.  progress.
+rewrite (drop_nth witness (size n{2} - 1)). smt(). simplify.
+rewrite /ith_bit. smt(@List).
+smt().
+rewrite hast2. smt(). rewrite H0. simplify.
+rewrite hast3. smt(). rewrite hast2. smt(). rewrite H0. rewrite prop1. simplify. rewrite /(^). simplify. smt.
+rewrite hast2. smt(). rewrite H0. simplify. auto.
+rewrite hast2. smt(). rewrite H0. auto.
+   rewrite hast2. smt(). rewrite H0. auto.
+   rewrite hast2. smt(). rewrite H0. auto.
+   rewrite hast2. smt(). rewrite H0. auto.
+ rewrite hast2. smt(). rewrite H0. auto.
+rewrite hast2. smt(). rewrite H0. auto.
+smt(). 
+have : ctr_L <= 0. smt().
+case (has_true (drop ctr_L n{2})).
+progress.
+rewrite H2. auto.
+have -> : (drop ctr_L n{2}) = n{2}. smt.
+auto.
+progress.
+have -> : x1_L = oneR. smt. 
+have y : !has_true n{2}. smt. 
+rewrite  hast4. auto. auto.
+qed.
