proof/examples/zk/abstract/Abstract_exp_proof_4.ec
@@ -1,0 +1,109 @@
+require import AllCore IntDiv CoreMap List.
+
+require import JModel.
+require import BitEncoding.
+import BS2Int.
+
+require import Abstract_exp_proof_1.
+require import Abstract_exp_proof_2.
+require import Abstract_exp_proof_3.
+
+
+import IterOp.
+
+module M4 = {
+
+    proc expm (x:R, n:R) : R = {
+    
+    var x1, x2, x3, x4, bit : R;
+    var par, p, d : W64.t;
+    var ctr:int;
+
+    d <- ith_bitR n (Rsize - 1);
+    (x1,x2,x3, x4) <- (oneR,oneR,x,x *** x);
+
+    ctr <- Rsize - 1;
+    p <- d;
+    (x1,x3) <- as_bool d ? (x3,x1) : (x1,x3);
+    (x2,x4) <- as_bool d ? (x4,x2) : (x2,x4);
+
+    while (0 < ctr) {
+      ctr <- (ctr - 1);
+      p <- d;
+      d <-  d `|` ith_bitR n ctr;
+      par <- ith_bitR n (ctr + 1) `^` ith_bitR n ctr;
+      (x1,x2) <- if as_bool par then (x2,x1) else (x1, x2);
+      x1 <- x1 *** x2;
+      x2 <- x2 *** x2;
+      (x1,x3) <- as_bool (d `^` p) ? (x3,x1) : (x1,x3);
+      (x2,x4) <- as_bool (d `^` p)  ? (x4,x2) : (x2,x4);
+    }
+    (x1,x2) <- if ! as_bool (ith_bitR n 0)  then (x2,x1) else (x1, x2);    
+    return x1;
+  }  
+
+
+}.
+
+
+
+lemma exp_3_4_1 :
+ equiv[ M3.expm ~ M4.expm : arg{1}.`1 = arg{2}.`1 /\ (bitsR arg.`2{1}) = (arg.`2{2})  /\ size n{1} = Rsize /\  0 < size n{1} ==> ={res}].
+proc.
+wp.
+while (={ctr,  x1,x2,  x3, x4, d, p}  
+   /\ bitsR n{1} = n{2}
+   /\ size n{1} = Rsize).
+wp. skip. progress. 
+smt (qqq www).
+smt (qqq www).
+smt (qqq www).
+smt (qqq www).
+smt (qqq www).
+wp. 
+skip. 
+progress.
+smt().
+smt (qqq www).
+smt (qqq www).
+smt (qqq www).
+smt (qqq www).
+smt (qqq www).
+smt (qqq www).
+smt().
+smt (qqq www).
+smt (qqq www).
+qed.
+
+
+
+lemma exp_3_4_2 :
+ equiv[ M3.expm ~ M4.expm : arg{1}.`1 = arg{2}.`1 /\ (arg.`2{1}) = (Rbits arg.`2{2})    /\  0 < size n{1} ==> ={res}].
+proc.
+wp.
+while (={ctr,  x1,x2,  x3, x4, d, p}  
+   /\ n{1} = Rbits n{2}
+   /\ size n{1} = Rsize).
+wp. skip. progress. 
+(* smt (qqq www). *)
+(* smt (qqq www). *)
+(* smt (qqq www). *)
+(* smt (qqq www). *)
+(* smt (qqq www). *)
+wp. 
+skip. 
+progress.  rewrite iii. auto.
+smt (qqq www iii).
+smt (qqq www iii).
+smt (qqq www iii).
+smt (qqq www iii).
+smt (qqq www iii).
+smt (qqq www iii).
+smt (qqq www iii).
+smt (qqq www iii).
+smt (qqq www iii).
+qed.
+
+
+
+
