proof/examples/zk/abstract/Abstract_exp_proof_5.ec
@@ -1,0 +1,66 @@
+require import AllCore IntDiv CoreMap List.
+
+require import JModel.
+require import BitEncoding.
+import BS2Int.
+
+require import Abstract_exp_proof_1.
+require import Abstract_exp_proof_2.
+require import Abstract_exp_proof_3.
+require import Abstract_exp_proof_4.
+
+import IterOp.
+
+
+module M5 = {
+
+  proc expm (x:R, n:R) : R = {
+    
+    var x1, x2, x3, x4, bit : R;
+    var t1,t2,par, p, d : W64.t;
+    var ctr: int;
+
+    d <@ Spec.ith_bit(n,  (Rsize - 1));
+    (x1,x2,x3) <- (oneR,oneR,x);
+    x4 <@ Spec.mul(x,x);
+
+    ctr <- Rsize - 1;
+    p <- d;
+    (x1,x3) <@ Spec.swapr (x1,x3,as_bool d);
+    (x2,x4) <@ Spec.swapr (x2,x4,as_bool d); 
+
+    while (0 < ctr) {
+      ctr <- (ctr - 1);
+      p <- d;
+      t1 <@ Spec.ith_bit(n,  (ctr + 1));
+      t2 <@ Spec.ith_bit(n, ctr);
+      d <-  d `|` t2;
+      par <- t1 `^` t2;
+      (x1,x2) <@ Spec.swapr (x1,x2,as_bool par); 
+      x1 <@ Spec.mul(x1,x2); 
+      x2 <@ Spec.mul(x2,x2);  
+      (x1,x3) <@ Spec.swapr (x1,x3,as_bool (d `^` p));  
+      (x2,x4) <@ Spec.swapr (x2,x4,as_bool (d `^` p));   
+    }
+    par <@ Spec.ith_bit(n,0);
+    (x1,x2) <@ Spec.swapr (x2,x1, as_bool par);
+    return x1;
+  }  
+}.
+
+
+lemma exp_4_5 :
+ equiv[ M4.expm ~ M5.expm  : ={arg} ==> ={res}].
+proc.
+inline Spec.mul.
+inline Spec.swapr.
+inline Spec.ith_bit.
+    wp.
+    wp.
+while (={ctr, n,  x1,x2,  x3, x4, d, p} ).
+ wp. skip. progress. 
+wp.  skip. progress. 
+smt().
+qed.
+
+
