proof/examples/zk/abstract/Abstract_exp_proof_6.ec
@@ -1,0 +1,109 @@
+require import AllCore IntDiv CoreMap List.
+
+require import JModel.
+require import BitEncoding.
+import BS2Int.
+
+require import Abstract_exp_proof_1.
+require import Abstract_exp_proof_2.
+require import Abstract_exp_proof_3.
+require import Abstract_exp_proof_4.
+require import Abstract_exp_proof_5.
+
+import IterOp.
+
+module M6(M : BasicOps) = {
+
+  proc expm (m : R, x:R, n:R) : R = {
+    
+    var x1, x2, x3, x4, bit : R;
+    var t1, t2, par, p, d : W64.t;
+    var ctr:int;
+
+    d <@ M.ith_bit(n,  W64.of_int (Rsize - 1));
+    (x1,x2,x3) <- (oneR,oneR,x);
+    x4 <@ M.mulm(m,x,x);
+
+    ctr <- Rsize - 1;
+    p <- d;
+    (x1,x3) <@ M.swapr(x1,x3,d);
+    (x2,x4) <@ M.swapr(x2,x4,d);
+
+    while (0 < ctr) {
+      ctr <- (ctr - 1);
+      p <- d;
+      t1 <@ M.ith_bit(n, W64.of_int (ctr + 1));
+      t2 <@ M.ith_bit(n, W64.of_int ctr);
+      d <-  d `|` t2;
+      par <- t1 `^` t2;
+      (x1,x2) <@ M.swapr(x1,x2,par);  
+      x1 <@ M.mulm(m,x1,x2); 
+      x2 <@ M.mulm(m,x2,x2);  
+      (x1,x3) <@ M.swapr(x1,x3,(d `^` p));
+      (x2,x4) <@ M.swapr(x2,x4,(d `^` p)); 
+    }
+    par <@ M.ith_bit(n,W64.of_int 0);
+    (x1,x2) <@ M.swapr (x2,x1,par);
+    return x1;
+  }  
+}.
+
+
+
+section.
+declare module M <: BasicOps.
+
+declare axiom exp_swap :
+ equiv[ M.swapr ~ Spec.swapr    : arg{2}.`1 = arg{1}.`1 /\ arg{2}.`2 = arg{1}.`2 /\   arg{1}.`3 = as_w64 arg{2}.`3
+    ==> ={res}].
+
+declare axiom exp_ithbit :
+ equiv[ M.ith_bit ~ Spec.ith_bit    : arg{2}.`1 = arg{1}.`1 /\  arg{2}.`2 = W64.to_uint arg{1}.`2 
+    /\ 0 <= ctr{2} < Rsize ==> ={res} /\ (res{2} = W64.one \/ res{2} = W64.zero) ].
+
+declare axiom exp_mulm : 
+  equiv [ M.mulm ~ Spec.mul: arg{1}.`2 = arg{2}.`1 /\ arg{1}.`3 = arg{2}.`2 /\   ImplR p{1} P  ==> ={res} ].
+
+    
+lemma exp_5_6 :
+ equiv[ M5.expm ~ M6(M).expm  : arg{2}.`2 = arg{1}.`1 /\ arg{2}.`3 = arg{1}.`2 /\   ImplR m{2} P ==> ={res}].
+symmetry.
+proc. 
+wp. 
+call exp_swap.
+call exp_ithbit.
+while ((d{2} = W64.one \/ d{2} = W64.zero) /\ ={ctr, n,  x1,x2,  x3, x4, d, p} /\ ImplR m{1} P /\  0 <= ctr{1} < Rsize).
+call exp_swap.
+call exp_swap.
+ wp. 
+call exp_mulm.
+call exp_mulm. 
+call exp_swap.
+wp. 
+call exp_ithbit.
+call exp_ithbit.
+wp.
+skip. 
+progress. smt. smt. smt(). smt().  smt(@W64).
+rewrite /as_word.
+rewrite /as_bool.  smt(@W64). smt(@W64).
+wp. 
+call exp_swap.
+call exp_swap.
+wp.
+call exp_mulm. 
+wp.
+call exp_ithbit. 
+skip.
+progress.
+rewrite /as_word.
+rewrite /as_bool.
+smt. smt(Rsize_pos). smt().
+rewrite /as_w64.
+rewrite /as_bool.
+smt().
+smt().
+smt().
+qed.
+
+end section.
