proof/examples/zk/abstract/Abstract_exp_proof_8.ec
@@ -1,0 +1,195 @@
+require import AllCore IntDiv CoreMap List.
+
+require import JModel.
+require import BitEncoding.
+import BS2Int.
+
+require import Abstract_exp_proof_1.
+require import Abstract_exp_proof_2.
+require import Abstract_exp_proof_3.
+require import Abstract_exp_proof_4.
+require import Abstract_exp_proof_5.
+require import Abstract_exp_proof_6.
+require import Abstract_exp_proof_7.
+
+import IterOp.
+import Zp.
+
+module M8 = {
+  proc expm_spec (x:R, n:R) : R = {
+    return (x ^ (valR n));
+  }  
+}.
+
+
+lemma iii : forall i, 0 <= i => forall  b,
+  iterop (i + 1) ( *** ) b oneR = b *** iterop i ( *** ) b oneR.
+apply intind.
+progress. smt.
+progress. 
+rewrite /iterop. 
+simplify. rewrite iteriS. auto. simplify. 
+have ->: (i + 2) = (i+1) + 1. smt().
+rewrite iteriS. smt().
+rewrite iteriS. smt().
+simplify. smt().
+qed.
+
+
+
+lemma kk :  forall (n : int), 0 <= n => forall (a : zp) (b : R),
+  ImplFp b a =>
+  ImplFp (b ^ n) (inzp (asint a ^ n)).
+apply intind. progress. 
+rewrite exp_prop1.
+have -> : (asint a ^ 0) = 1. smt.
+rewrite /asint.
+have -> : (Sub.val (inzp 1))%Sub = 1. smt.
+smt(valR_one).
+progress.
+have ->: (b ^ (i + 1)) = b *** (b ^ i).
+rewrite exp_prop3. 
+rewrite exp_prop2.
+rewrite exp_prop7. auto.
+have ->: inzp (asint a ^ (i + 1)) =  inzp (asint a * (asint a ^ i)).
+smt.
+have ->:  inzp (asint a * (asint a ^ i)) = (inzp (asint a)) * (inzp (asint a ^ i)).
+smt.
+rewrite - H1.
+have ->: asint (inzp (valR b) * inzp (valR b ^ i))
+  = (asint (inzp (valR b)) * (asint  (inzp (valR b ^ i)))) %% P.
+smt.
+have ih :  ImplFp (b ^ i)  (inzp (valR b ^ i)).
+rewrite H1. apply H0. auto.
+rewrite - ih.
+have ->: asint (inzp (valR b)) = valR b. smt.
+have ->: valR (b *** (b ^ i)) =  (valR b) * (valR (b ^ i)) %%P.
+rewrite  to_uintP /=. done.
+auto.
+qed.
+
+
+lemma exp_real_speacc :
+ equiv[ Spec.expm ~ M8.expm_spec  : 
+    ImplFp arg{2}.`1 arg{1}.`1 /\ valR arg{2}.`2 = arg{1}.`2 ==> ImplFp res{2} res{1}].
+proc. 
+wp.  skip.  progress.
+apply kk.
+smt.
+auto.
+qed.
+
+
+lemma exp_real_speac2 :
+ equiv[ M8.expm_spec ~ M1.expm_spec   : arg{1}.`1 = arg{2}.`1 /\  valR arg{1}.`2 = tonat arg{2}.`2 ==> ={res}] .
+proc. skip. progress.
+smt().
+qed.
+
+
+
+section.
+declare module M <: BasicOps.
+
+declare axiom exp_swap :
+ equiv[ M.swapr ~ Spec.swapr    : arg{2}.`1 = arg{1}.`1 /\ arg{2}.`2 = arg{1}.`2 /\   arg{1}.`3 = as_w64 arg{2}.`3
+    ==> ={res}].
+
+declare axiom exp_ithbit :
+ equiv[ M.ith_bit ~ Spec.ith_bit    : arg{2}.`1 = arg{1}.`1 /\  arg{2}.`2 = W64.to_uint arg{1}.`2 
+    /\ 0 <= ctr{2} < Rsize ==> ={res} /\ (res{2} = W64.one \/ res{2} = W64.zero) ].
+
+declare axiom exp_mulm : 
+  equiv [ M.mulm ~ Spec.mul: arg{1}.`2 = arg{2}.`1 /\ arg{1}.`3 = arg{2}.`2 /\   ImplR p{1} P  ==> ={res} ].
+
+declare axiom stateless_M (x y : glob M) : x = y.
+
+lemma exp_real_speac :
+ equiv[ M1.expm_spec ~ M7(M).expm  : valR arg{2}.`1 = P 
+   /\  arg{1}.`1 = arg{2}.`2
+   /\ tonat arg{1}.`2 = valR arg{2}.`3
+   /\ size arg{1}.`2 = Rsize
+     ==> ={res}].
+transitivity M2.expm
+   (={arg} /\  0 < size arg{1}.`2 ==> ={res}) 
+  (valR arg{2}.`1 = P 
+   /\  arg{1}.`1 = arg{2}.`2
+   /\ tonat arg{1}.`2 = valR arg{2}.`3
+   /\ size arg{1}.`2 = Rsize
+     ==> ={res} ).
+progress.  exists arg{1}. progress. smt(Rsize_pos). auto.
+symmetry.
+conseq expm_correct.
+auto. auto.
+transitivity M3.expm
+  (={arg} /\  0 < size n{1} ==> ={res})
+  (valR arg{2}.`1 = P 
+   /\  arg{1}.`1 = arg{2}.`2
+   /\ tonat arg{1}.`2 = valR arg{2}.`3
+   /\ size arg{1}.`2 = Rsize
+     ==> ={res} ).
+progress. 
+exists arg{1}. progress. smt(Rsize_pos). auto.
+conseq exp_2_3.
+transitivity M4.expm
+  (arg{1}.`1 = arg{2}.`1 /\ (bitsR arg.`2{1}) = (arg.`2{2})  /\ size n{1} = Rsize /\  0 < size n{1} ==> ={res})
+(valR arg{2}.`1 = P 
+   /\  arg{1}.`1 = arg{2}.`2
+   /\ arg{1}.`2 = arg{2}.`3
+     ==> ={res} ).
+progress. 
+exists (x{1} , ( n{2})). progress. 
+smt (bitsR_prop).
+smt(Rsize_pos). auto.
+conseq exp_3_4_1.  progress.
+  
+transitivity M5.expm
+  (={arg} ==> ={res})
+  (valR arg{2}.`1 = P 
+   /\  arg{1}.`1 = arg{2}.`2
+   /\ arg{1}.`2 = arg{2}.`3
+     ==> ={res} ).
+progress. 
+exists (x{1} , ( n{2})). progress.  smt(). auto.
+conseq exp_4_5.  
+transitivity M6(M).expm
+ (arg{2}.`2 = arg{1}.`1 /\ arg{2}.`3 = arg{1}.`2 /\  valR m{2} = P ==> ={res})
+  (={arg} ==> ={res}).
+progress. smt(). smt().
+conseq (exp_5_6 M exp_swap exp_ithbit exp_mulm). 
+conseq (exp_6_7 M).
+smt (stateless_M).
+qed.
+
+
+lemma exp_pre_fin :
+ equiv[ Spec.expm ~ M7(M).expm  : valR arg{2}.`1  = P 
+   /\  ImplFp  arg{2}.`2 arg{1}.`1
+   /\ arg{1}.`2 =  valR arg{2}.`3
+     ==> ImplFp res{2} res{1} ].
+transitivity M8.expm_spec
+  (ImplFp arg{2}.`1 arg{1}.`1 /\ valR arg{2}.`2 = arg{1}.`2 ==> ImplFp res{2} res{1})
+  (valR arg{2}.`1 = P 
+   /\  arg{1}.`1 = arg{2}.`2
+   /\  arg{1}.`2 =  arg{2}.`3
+     ==> ={res}).
+progress. exists (x{2},n{2}). progress. smt(). auto.
+conseq exp_real_speacc.   
+transitivity M1.expm_spec  
+  (arg{1}.`1 = arg{2}.`1 /\ valR arg{1}.`2 = tonat arg{2}.`2 ==> ={res})
+  (valR arg{2}.`1 = P 
+   /\  arg{1}.`1 = arg{2}.`2
+   /\ tonat arg{1}.`2 = valR arg{2}.`3
+   /\ size arg{1}.`2 = Rsize
+     ==> ={res}).
+progress. 
+exists (x{1},  Rbits n{2}).
+progress.
+smt().
+smt(rsize_prop).
+smt().
+conseq exp_real_speac2. 
+conseq exp_real_speac.
+qed.
+
+end section.
