proof/examples/zk/multlimb/W64_exp_proof_2.ec
@@ -1,0 +1,80 @@
+require import AllCore IntDiv CoreMap List.
+
+require import JModel.
+require import BitEncoding.
+import BS2Int.
+
+require import Zp_big.
+require import W64_exp_proof_1.
+
+import Zp.
+import IterOp.
+
+
+
+module M2 = {
+
+    proc expm (x:R, n:bits) : R = {
+    
+    var x1, x2, x3, x4 : R;
+    var ctr:int;
+    var bit, d, p, par :bool;    
+    d <- ith_bit n (size n - 1);
+    (x1,x2,x3, x4) <- (oneR,oneR,x,x *** x);
+
+    ctr <- size n - 1;
+    p <- d;
+    (x1,x3) <- d ? (x3,x1) : (x1,x3);
+    (x2,x4) <- d ? (x4,x2) : (x2,x4);
+
+    while (0 < ctr) {
+      ctr <- (ctr - 1);
+      p <- d;
+      d <- d || ith_bit n ctr;
+      par <- ith_bit n (ctr + 1) ^ ith_bit n ctr;
+      (x1,x2) <- if par then (x2,x1) else (x1, x2);
+      x1 <- x1 *** x2;
+      x2 <- x2 *** x2;
+      (x1,x3) <- d ^ p ? (x3,x1) : (x1,x3);
+      (x2,x4) <- d ^ p ? (x4,x2) : (x2,x4);
+    }
+    (x1,x2) <- if ! ith_bit n 0 then (x2,x1) else (x1, x2);    
+    return x1;
+  }  
+
+
+}.
+
+
+lemma exp_eq_naive :
+ equiv[ M1.expm_naive ~ M2.expm : ={arg} /\  0 < size n{1} ==> ={res}].
+proc.
+wp.
+while (={ctr, n, d, p, x3, x4} /\ 0 < ctr{2} + 1 <= size n{2}
+   /\ (ith_bit n{2} (ctr{2}  ) => x2{2} = x2{1} /\ x1{2} = x1{1})
+   /\ ((!ith_bit n{2} (ctr{2} ) ) => (x1{1} = x2{2} /\ x2{1} = x1{2}))
+   ).
+wp. skip. progress. smt().     smt. smt.
+rewrite H5. simplify. smt().
+rewrite H5. simplify. smt().
+rewrite H5. simplify. smt().
+rewrite H5. simplify. smt().
+wp.  
+skip. progress. smt(). smt(). 
+smt().
+qed.
+
+
+
+lemma expm_correct : 
+  equiv[ M2.expm ~ M1.expm_spec : ={arg} /\  0 < size arg{1}.`2 ==> ={res}].
+transitivity M1.expm_naive 
+  (={arg}  /\  0 < size arg{1}.`2 ==> ={res})
+  (={arg}  /\  0 < size arg{1}.`2 ==> ={res}).
+smt().
+auto. symmetry.
+conseq exp_eq_naive. auto. auto.
+exists* n{1}, x{1}. elim*. progress.
+conseq (exp_naive_correct f0 f). progress. smt().
+qed.
+
